

Assignment 5

Yiyun Zhang

1. Prove $\sum_{i=1}^n ba_i = b \sum_{i=1}^n a_i$

Base case: If $n = 1$, $\sum_{i=1}^1 ba_i = ba_1 = b \sum_{i=1}^1 a_i$

General case:

Inductive Hypothesis: $\sum_{i=1}^n ba_i = b \sum_{i=1}^n a_i$

Show: $\sum_{i=1}^{n+1} ba_i = b \sum_{i=1}^{n+1} a_i$

$$\begin{aligned}\sum_{i=1}^{n+1} ba_i &= \sum_{i=1}^n ba_i + ba_{n+1} \\ &= b \sum_{i=1}^n a_i + ba_{n+1} \\ &= b \left(\sum_{i=1}^n a_i + a_{n+1} \right) \\ &= b \sum_{i=1}^{n+1} a_i\end{aligned}$$

Therefore $\sum_{i=1}^n ba_i = b \sum_{i=1}^n a_i$

Prove $\sum_{i=1}^n (a_i + b_i) = \sum_{i=1}^n a_i + \sum_{i=1}^n b_i$

Base case: If $n = 1$, $\sum_{i=1}^1 (a_i + b_i) = a_1 + b_1 = \sum_{i=1}^1 a_i + \sum_{i=1}^1 b_i$

General case:

Inductive Hypothesis: $\sum_{i=1}^n (a_i + b_i) = \sum_{i=1}^n a_i + \sum_{i=1}^n b_i$

Show: $\sum_{i=1}^{n+1} (a_i + b_i) = \sum_{i=1}^{n+1} a_i + \sum_{i=1}^{n+1} b_i$

$$\begin{aligned}\sum_{i=1}^{n+1} (a_i + b_i) &= \sum_{i=1}^n (a_i + b_i) + (a_{n+1} + b_{n+1}) \\ &= \sum_{i=1}^n a_i + \sum_{i=1}^n b_i + (a_{n+1} + b_{n+1})\end{aligned}$$

$$\begin{aligned}
&= \left(\sum_{i=1}^n a_i + a_{n+1} \right) + \left(\sum_{i=1}^n b_i + b_{n+1} \right) \\
&= \sum_{i=1}^{n+1} a_i + \sum_{i=1}^{n+1} b_i
\end{aligned}$$

Therefore $\sum_{i=1}^n (a_i + b_i) = \sum_{i=1}^n a_i + \sum_{i=1}^n b_i$

2. $F_n = F_{n-1} + F_{n-2}$, $F_0 = 0$, $F_1 = 1$
Find m that $F_m > (3/2)^m$

| n | F_n | $(3/2)^n$ |
|----|-------|-------------|
| 0 | 0 | 1 |
| 1 | 1 | 1.5 |
| 2 | 1 | 2.25 |
| 3 | 2 | 3.375 |
| 4 | 3 | 5.0625 |
| 5 | 5 | 7.59375 |
| 6 | 8 | 11.390625 |
| 7 | 13 | 17.0859375 |
| 8 | 21 | 25.62890625 |
| 9 | 34 | 38.44335938 |
| 10 | 55 | 57.66503906 |
| 11 | 89 | 86.49755859 |
| 12 | 144 | 129.7463379 |
| 13 | 233 | 194.6195068 |

From the table we can get when $n = 11$, the value of $F_n > (3/2)^n$, so 11 is the smallest non-negative integer.

Prove $F_n > (3/2)^n$ for all values of $n > 11$

Base case: If $n = 11$, $F_n > (3/2)^n$ is true by last step.

General case:

Inductive hypothesis: $F_n > (3/2)^n$, $F_{n-1} > (3/2)^{n-1}$

Show: $F_{n+1} > (3/2)^{n+1}$

$$\begin{aligned} F_{n+1} &= F_n + F_{n-1} > (3/2)^n + (3/2)^{n-1} \\ &= F_n + F_{n-1} > (3/2)^n + (3/2)^n * (3/2)^{-1} \\ &= F_n + F_{n-1} > (3/2)^n * (1 + 2/3) \\ &= F_n + F_{n-1} > (3/2)^n * (5/3) \\ &= F_n + F_{n-1} > (3/2)^{n+1} * (2/3) * (5/3) \\ &= F_n + F_{n-1} > (3/2)^{n+1} * (10/9) \end{aligned}$$

Since $10/9 > 1$, so $(3/2)^{n+1} * (10/9) > (3/2)^{n+1}$, and $F_{n+1} > (3/2)^{n+1} * (10/9) > (3/2)^{n+1}$.

Therefore $F_n > (3/2)^n$ for all values of $n > 11$

3. Prove a truth table with n variables has 2^n rows

Base case: If $n = 1$, the truth table has 2 rows (T and F). which is 2^1 .

General case:

Inductive hypothesis: a truth table with n variables has 2^n rows.

Show: a truth table with $n+1$ variables has 2^{n+1} rows

Since a truth table with n variables has 2^n rows. The extra variable in $n+1$ has two copies of the table of with n variables (T for one copy and F for another copy). Therefore the total number of rows of $n+1$ variables table is $2 * 2^n = 2^{n+1}$.

4. Let $x_1 \dots x_n$ be binary variables. Prove $\text{parity}(x_1 \dots x_n) = x_1 \oplus \dots \oplus x_n$

Base case: If $n = 1$, $\text{parity}(0) = 0$, $\text{parity}(1) = 1$, therefore $\text{parity}(x) = x$.

General case:

Inductive hypothesis: $x_1 \oplus \dots \oplus x_n = \text{parity}(x_1 \dots x_n)$

Show: $x_1 \oplus \dots \oplus x_{n+1} = \text{parity}(x_1 \dots x_n) \oplus x_{n+1}$

If $x_{n+1} = 0$, $\text{parity}(x_1 \dots x_n) \oplus 0$, Since $x \oplus 0 = x$, $\text{parity}(x_1 \dots x_n, 0) = \text{parity}(x_1 \dots x_n)$
 $\text{parity}(x_1 \dots x_n) \oplus x_{n+1} = \text{parity}(x_1 \dots x_{n+1})$

If $x_{n+1} = 1$, $\text{parity}(x_1 \dots x_n) \oplus 1$, Since $x \oplus 1 = c$ (complement of x)
 $\text{parity}(x_1 \dots x_n, 1) = \overline{\text{parity}(x_1 \dots x_n)}$ (complement of $\text{parity}(x_1 \dots x_n)$)

5. Prove $G_n = [0G_{n-1}, 1G'_{n-1}]$ is gray code

Base case: If $n = 1$, $[0..2^1-1] = [0..1]$, which is a gray code.

General case:

Inductive hypothesis: G_{n-1} is a gray code

Show: $G_n = [0G_{n-1}, 1G'_{n-1}]$ is a gray code

Since G_{n-1} is a gray code, $0G_{n-1}$, $1G_{n-1}$ and G'_{n-1} are gray code. Since the last element of G_{n-1} is the same as the first element of G'_{n-1} , so the last element of $0G_{n-1}$ and the first element of $1G'_{n-1}$ differ by exactly one bit.

Therefore $G_n = [0G_{n-1}, 1G'_{n-1}]$ is a gray code.

6. Prove $G_n(i), i=0, \dots, 2^n-1 = [G_n(0) \dots G_n(2^n-1)]$ is a binary-reflected gray code

Base case: If $n = 1$, $G_1(i)=[G_1(0), G_1(1)] = [0, 1]$, which is a gray code.

General case:

Inductive hypothesis: $G_n = [G_n(0) \dots G_n(2^n-1)]$ is a binary-reflected gray code

Show: $G_{n+1} = [G_{n+1}(0) \dots G_{n+1}(2^{n+1}-1)]$ is a binary-reflected gray code

$[G_{n+1}(0) \dots G_{n+1}(2^{n+1}-1)] =$